\documentclass[11pt]{article}
\usepackage{amssymb}
\usepackage{fullpage}
\setlength{\parskip}{1ex}
\setlength{\parindent}{0in}
\def\nats {{\mathbb N}}
\def\ints {{\mathbb Z}}

\usepackage{comment}
\includecomment{solution}
\excludecomment{question}
\newcommand{\Implies}{\mbox{ IMPLIES }}
\newcommand{\Or}{\mbox{ OR }}
\newcommand{\And}{\mbox{ AND }}
\newcommand{\Not}{\mbox{ NOT }}
\newcommand{\Iff}{\mbox{ IFF }}
\newcommand{\True}{\mbox{T}}
\newcommand{\False}{\mbox{F}}

\begin{document}

{\bf \large Quiz 7}

\medskip

\begin{question}
Solve the recurrence
$$A(n) = \left \{
\begin{array}{ll}
1 & \mbox{if } n = 1\\
n^2A(n-1)  & \mbox{if } n \geq 2
\end{array} \right .$$
using any technique except looking up the answer.
\end{question}

\begin{solution}
{\bf Solution}:\\
Solving by plug and chug:\\
$$A(n)= 2^n \cdot A(n-1)=)=$$
$$=2^n \cdot 2^{n-1} \cdot A(n-2) =$$
$$=2^n \cdot 2^{n-1} \cdot 2^{n-2} \cdot A(n-3)= $$
$$=2^n \cdot 2^{n-1} \cdot 2^{n-2} \cdot 2^{n-3} \cdot A(n-4)= $$
$$= 2^{4n-6} A(n-4)$$
Assume that $n-4 =1$ therefore $n=5$ and $A(n-4) = 1$\\
$$ A(5)= 2^{(5-1)5-6}$$
With this repeated substitution, it seems as if the final sum is $2^{n(n-1) - x}$ where $x$ is the sum of every positive integer 1 less than $n$\\
Since the sum of all integers less than an arbitrary number $y$ is $\frac{y(y-1)}2$, and since in this case $y=n-1$\\
$$x = \frac{(n-1)(n-1-1)}2 =  \frac{(n-1)(n-2)}2$$\\
Theroretically the final sum can be represented as \\
$$ A(n) = 2^{n(n-1) - (n-1)(n-2)/2}$$\\
{\bf Proof by induction:}\\
{\bf Definitions:}\\
$P(n) \nats\rightarrow \{T,F\} ::= A(a) = 2^{n(n-1) - (n-1)(n-2)/2} $\\
Claim $\forall a\in A. P(a)$\\
{\bf Base case: }\\
$A(1) =1 $ by the definition of the function $A$\\
$2^{1(1-1) - (1-1)(1-2)/2 = 2^0 = 1}$\\
Therefore $A(a)$ holds for the base case\\
{\bf Induction Step:}\\
\null\quad Let $a\in A$ be arbitrary.\\
\null\qquad Assume $P(a)$ (I.H)\\
\null\qquad Therefore $A(a-1) = 2^{(a-1)((a-1)-1) - ((a-1)-1)((a-1)-2)/2} = 2^{(a-1)(a-2) - (a-2)(a-3)/2}$\\
\null\qquad By the definition of $A$: $A(a) = 2^n + A(a-1)$\\
\null\qquad $=2^a \cdot 2^{(a-1)(a-2) - (a-2)(a-3)/2}  =2^{a(a-1) - (a-1)(a-2)/2}  $\\
\null\quad Therefore $P(a-1) \Implies P(a)$\\
Therefore by induction $\forall a\in \nats.P(a)$\\

\end{solution}
\end{document}
