\documentclass[11pt]{article}
\usepackage{amssymb}
\usepackage{fullpage}
\pagestyle{empty}
\setlength{\parskip}{1ex}
\setlength{\parindent}{0in}
\usepackage{comment}


\def\nats{{\mathbb N}}
\def\ints{{\mathbb Z}}
\includecomment{solution}
\includecomment{question}
\setlength{\parskip}{1ex}
\newcommand{\Implies}{\mbox{ IMPLIES }}
\newcommand{\And}{\mbox{ AND }}
\newcommand{\Iff}{\mbox{ IFF }}
\newcommand{\Or}{\mbox{ OR }}
\newcommand{\Not}{\mbox{NOT }}

\begin{document}

{\bf \large Quiz 4}

\begin{question}
The Fibonacci sequence
$$0,1,1,2,3,5,8,12,21, \ldots$$
starts with the numbers 0 and 1 and each successive element is the sum of the two previous elements.
This sequence can be written as
$$F(0), F(1), F(2), \ldots$$
where
$F:\nats \rightarrow \nats$ is defined
as follows:\\
$F(0) = 0$,\\
$F(1) = 1$, and\\
for all $n \geq 2$, $F(n) = F(n-1) + F(n-2)$.


Prove by induction that,  for all nonnegative integers $n$,
$$F(n)  = \frac{a^n -b^n}{\sqrt{5}}$$
where $a = (1+\sqrt{5})/2$ and $b = (1-\sqrt{5})/2$ are the roots of the equation $x^2 - x -1 =0$.\\
\end{question}
\begin{solution}
{\bf Solution}:\\
{\bf{Claim}}: $\forall n\in N_{\ge1}.Q(n)$. Where $Q(n): N\rightarrow \{T,F\} = \left (n = \frac{a^n - b^n}{\sqrt 5}\right )$. Where: $a=\frac{1+\sqrt 5}{2},$ $b=\frac{1+\sqrt 5}{2}$\\\\
{\bf Cases:}\\
\null\quad$Q(1):\frac{a^1-b^1}{\sqrt 5} = \frac{(1+\sqrt 5) - (1-\sqrt 5)}{2\sqrt 5} = \frac{2\sqrt 5}{2\sqrt 5}= 1 = F(1)$. Therefore $Q(1)$ holds\\\\
\null\quad$Q(2):\frac{a^2-b^2}{\sqrt 5} = \frac{(\frac{1+\sqrt 5}{2})^2 - (\frac{1-\sqrt 5}{2})^2}{\sqrt 5}= \frac{(1 + 2\sqrt 5 + 5)- (1-2\sqrt 5 + 5)}{4\sqrt 5} = \frac{4\sqrt 5}{4\sqrt 5} = 1 = F(2)$.\\\\
\null\qquad Therefore $Q(2)$ holds\\\\
{\bf Induction hypothesis}: Let $k\ge1$ be an integer and assume that $Q(i)$ is true  for any value \\\null\quad $1\le i\le k$\\\\
\null\quad$Q(k).k\ge3$: By the I.H, and since $k\ge3$, it follows that $Q(k-1)$ and $Q(k-2)$ both hold\\
\null\qquad true.\\
\null\qquad Therefore $F(k-1) = \frac{a^{k-1}-b^{k-1}}{\sqrt 5}$ and $F(k-2) = \frac{a^{k-2}-b^{k-2}}{\sqrt 5}$\\
\null\qquad Since by the definition of the fibonacci sequence, $F(k) = F(k-1) + F(k-2)$, it follows that\\\\
\null\qquad $F(k) = \frac{a^{k-1}-b^{k-1}}{\sqrt 5} + \frac{a^{k-2}-b^{k-2}}{\sqrt 5} = \frac{((\frac{1+\sqrt 5}{2})^{k-1}-(\frac{1-\sqrt 5}{2})^{k-1}) + ((\frac{1+\sqrt 5}{2})^{k-2}-(\frac{1-\sqrt 5}{2})^{k-2})}{\sqrt 5} = \frac{\frac{1+\sqrt 5}{2}^k -\frac{1-\sqrt 5}{2}^k}{\sqrt 5}=\\$
\null\qquad $\frac{a^k -b^k}{\sqrt 5}$: Therefore $Q(k)$ holds true.\\\\
By induction $\forall n\in N_{\ge1}.Q(n)$

\end{solution}
\end{document}
